coq/_vc/Concordium_Prims.v
@@ -7,6 +7,7 @@ Open Scope Z_scope.
 Open Scope bool_scope.
 Open Scope hacspec_scope.
 Require Import Hacspec_Lib.
+Export Hacspec_Lib.
 
 Definition accept_hacspec   : int32 :=
   @repr WORDSIZE32 (1).
